Especificaciones/Clique/Clique.dfy
@@ -1,0 +1,10 @@
+include "../Auxiliar/Graph.dfy"
+
+predicate isClique(g: Graph, I: set<Node>)
+    requires isValidGraph(g)
+{
+    I <= g.0 && forall a, b: Node | a in I && b in I && a != b :: {a, b} in g.1
+}
+
+
+
