Especificaciones/Clique/CliqueOpt.dfy
@@ -1,0 +1,22 @@
+include "Clique.dfy"
+
+ghost predicate CliqueDecissionProblem(g: Graph, k: nat)
+    requires isValidGraph(g)
+{
+    exists I: set<Node> :: isClique(g, I) && |I| >= k
+}
+
+ghost predicate optimalValueClique(g: Graph, k: nat)
+    requires isValidGraph(g)
+{
+    CliqueDecissionProblem(g, k) 
+   && forall x: nat | CliqueDecissionProblem(g, x) :: x <= k
+}
+
+ghost predicate optimalClique(g: Graph, I: set<Node>)
+    requires isValidGraph(g)
+{
+       I <= g.0 
+    && isClique(g, I) 
+    && forall S: set<Node> | S <= g.0 && isClique(g, S) :: |S| <= |I|
+}
