Turing Reducciones/Clique/PCToPDC.dfy
@@ -1,0 +1,40 @@
+include "../../Especificaciones/Clique/CliqueOpt.dfy"
+include "../../Especificaciones/Clique/CliqueProperties.dfy"
+
+
+
+//We assume a polynomial algorithm for PDC
+method {:axiom} mCliqueDecissionProblem (graph : Graph, k : nat) returns (b : bool)
+  requires isValidGraph(graph)
+  ensures b == CliqueDecissionProblem(graph, k)
+
+//We implement a polynomial algorithm for PC using mCliqueDecissionProblem
+method mOptimalValueClique (graph : Graph) returns (k : nat)
+  requires isValidGraph(graph)
+  ensures optimalValueClique(graph,k)
+{
+  //If the graph is empty, the largest clique is an empty set
+  if graph.0 == {} {
+    k := 0;
+  }
+  else{
+    //We iterate from 0 to the number of vertices looking for the largest Clique we can find
+    var idx: nat := 1;
+    var notDone: bool := true;
+    LowerBoundClique(graph);
+    UpperBoundClique(graph);
+    while notDone
+        decreases |graph.0| - idx + 2
+        invariant 1 <= idx <= |graph.0| + 2
+        invariant (idx == |graph.0| + 2) ==> !notDone
+        invariant notDone ==> forall a: nat | 0 <= a < idx :: CliqueDecissionProblem(graph, a)
+        invariant !notDone ==> forall a: nat | idx  - 1 <= a <= |graph.0| :: !CliqueDecissionProblem(graph, a) 
+        invariant !notDone ==> forall a: nat | 0 <= a < idx - 1 :: CliqueDecissionProblem(graph, a)
+        invariant !notDone ==> idx >= 2
+    {
+        notDone := mCliqueDecissionProblem(graph, idx);
+        idx := idx + 1;
+    }
+    k := idx - 2;
+  }
+}
