Turing Reducciones/Clique/PDCToPOC.dfy
@@ -1,0 +1,19 @@
+include "../../Especificaciones/Clique/CliqueOpt.dfy"
+include "../../Especificaciones/Clique/CliqueProperties.dfy"
+
+
+
+//We assume a polynomial algorithm for POC
+method {:axiom} mOptimalClique (graph : Graph) returns (I: set<Node>)
+  requires isValidGraph(graph)
+  ensures optimalClique(graph, I)
+
+//We implement a polynomial algorithm for PDC using mOptimalClique
+method mOptimalValueClique (graph : Graph, k: nat) returns (b: bool)
+  requires isValidGraph(graph)
+  ensures b == CliqueDecissionProblem(graph,k)
+{
+  var optClique: set<Node> := mOptimalClique(graph);
+  assert isClique(graph, optClique);
+  b := (|optClique| >= k);
+}
