Turing Reducciones/Clique/POCToPC.dfy
@@ -1,0 +1,146 @@
+include "../../Especificaciones/Clique/CliqueOpt.dfy"
+include "../../Especificaciones/Clique/CliqueProperties.dfy"
+/*
+ghost predicate invariantLoop(
+  graph : Graph, okg : nat,
+  vertex : set<Node>,//remaining vertex
+  I : set<Node>, //up to now vertex cover
+  g : Graph, kg : nat//current graph
+)
+{ true }
+*/
+
+
+ghost predicate invariantLoop(
+  graph : Graph, okg : nat,
+  vertex : set<Node>,//remaining vertex
+  I: set<Node>, 
+  g : Graph, kg : nat//current graph
+)
+requires isValidGraph(graph)
+{
+  //g is a valid subgraph of graph
+  isValidGraph(g) &&
+  isSubGraph(g, graph) &&
+  okg >= 1 &&
+  kg == okg &&
+  //g has at leat okg vertices
+  |g.0| >= okg &&
+  //while g has more than okg vertices, vertex is not empty
+  (|g.0| > okg ==> vertex != {}) &&
+  //the partial solution is subset of the vertices in g
+  I <= g.0 &&
+  //vertices that have not been analyzed are a subset of the vertices in g
+  vertex <= g.0 &&
+  //all vertices in the partial solution have been analyzed
+  I == g.0 - vertex &&
+  //TODO expresar esto de una mejor manera
+  //forall node: Node | node in I :: optimalValueClique(removeVertex(g, node), kg - 1)  &&
+  optimalValueClique(g, okg) && 
+  //I is a prtial solution
+  //DEJAR SIN COMENTAR
+  (exists S: set<Node> :: S <= g.0 && optimalClique(graph, S) && I <= S) 
+
+  //g.1 +  (set edge:Edge, node:Node | edge in graph.1 && node in I && node in edge :: edge) == graph.1 &&
+
+  //At the end kg = 0 and |I| = okg, so I is optimal
+  //kg >= 0 && optimalValueVertexCover(g,kg) &&
+  //kg + |I| == okg //&&
+
+  //(forall u, O | u in g.0 && u !in vertex &&  I <= O <= graph.0 && isClique(graph, O) && |O| == okg :: u !in O) &&
+  //exists V : set<Node> :: V <= g.0 && optimalClique(graph, V) //&& optimalVertexCover(graph, I + V))
+}
+
+
+
+//We assume a polynomial algorithm for PCV
+method {:axiom} moptimalValueClique (graph : Graph) returns (k: nat)
+  requires isValidGraph(graph)
+  ensures optimalValueClique(graph,k)
+
+//We implement a polynomial algorithm for PDCV using moptimalVertexCover
+method mOptimalClique (graph:Graph) returns (I:set<Node>)
+  requires isValidGraph(graph)
+  ensures optimalClique(graph, I)
+{
+  if graph.0 == {} { I := {}; }
+  else {
+    I := {};
+    //this is the initial set of vertex
+    //used to traverse the graph vertices
+    var vertex := graph.0; 
+    //Optimal Clique value for graph
+    var okg :=  moptimalValueClique(graph);
+    UpperBoundClique(graph);
+    assert okg <= |graph.0|; 
+    //Current graph, it contains nodes that have not been analyzed and nodes which have been analyzed to belong to an optimal Clique for graph
+    var g := graph; 
+    //Optimal Clique value for the current graph
+    var kg := moptimalValueClique(g);
+
+    CliqueTranslation(g, kg);
+    nonEmptyClique(g);
+
+    //stop when g.0 == I
+    while (|I| < okg)
+      decreases vertex
+      invariant invariantLoop(graph,okg,vertex,I,g,kg)
+    {  
+      //UpperBoundClique(graph);
+      var v: Node := pick(vertex);
+      //Remove vertex v
+      var g' := removeVertex(g, v); 
+      validSubgraph(g,v,g');
+      var kg': nat := moptimalValueClique(g');
+
+      //Only two options are possible
+      assert kg' == kg || kg == kg' + 1 by { ovCliqueRemoveVertex(g, g', v, kg, kg'); } 
+      if kg == kg' + 1 
+      { 
+        //any optimal clique for g must include v
+        
+        isPartialSolutionWith1(g, g', v, kg, kg', I);
+        assert forall S: set<Node> | S <= g.0 && optimalClique(g, S) :: v in S;
+        //esta demostración noes trivial
+        
+        /*
+        ///////////
+        var fooNode: Node := pick(I);
+        var fooGraph: Graph := removeVertex(g, fooNode);
+        var fooNat: nat := moptimalValueClique(fooGraph);
+        assert fooNat + 1== kg;
+        assume{:axiom} false;
+        ///////////
+      */
+
+        assert forall node: Node | node in I :: (forall S: set<Node> | S <= g.0 && optimalClique(g, S) :: node in S);
+        assume{:axiom} false;
+        assert isClique(g, I) by 
+        {
+          assert exists S: set<Node> :: S <= g.0 && optimalClique(g, S);
+          var S: set<Node> :| S <= g.0 && optimalClique(g, S);
+          assert forall node: Node | node in I :: node in S;
+        }
+        
+        isPartialSolutionWith(g, g', v, kg, kg', I);
+        I := I + {v};
+        
+      }
+      //there exists an optimal clique that does not contain v
+      else { //kg == kg'
+        ghost var S: set<Node> :| S <= g'.0 && optimalClique(g', S);
+        CliqueInSubgraph(graph, g', kg, S);
+        isPartialSolutionWithout(g, g', v, kg, kg', I);
+        g := g';  
+        //TODO must prove it does not belong to some partial solution
+      }
+      vertex := vertex - {v};
+      assert exists S: set<Node> :: S <= g.0 && optimalClique(graph, S) && I <= S;
+      ghost var S: set<Node> :| S <= g.0 && optimalClique(graph, S) && I <= S;
+      cardinalityLemma3(S, g.0);
+      assert |g.0| >= |S|;
+      CliqueTranslation(g, kg);
+    }
+    cardinalityLemma2();
+  }
+}
